reduction_directedHamiltonianCircuit_to_hamiltonianCircuit/reduction_hamiltonian_rCompletness.dfy
@@ -1,0 +1,293 @@
+include "reduction_hamiltonian_definitions.dfy"
+include "reduction_hamiltonian_rFunction.dfy"
+
+module ReductionCompletness
+{
+    import opened Definitions
+    import opened ReductionFunction
+
+    ///// REDUCTION COMPLETNESS /////
+
+    lemma reduction_lemma(g: Graph)
+        requires validGraph(g)
+        ensures directedHamiltonianCircuit(g) <==> undirectedHamiltonianCircuit(directed_to_undirected_graph(g))
+    {
+        if directedHamiltonianCircuit(g)
+        {
+            reduction_lemma_right(g);
+        }
+        if undirectedHamiltonianCircuit(directed_to_undirected_graph(g))
+        {
+            reduction_lemma_left(g);
+        }
+    }
+
+    // Reduction to the right: directedHamiltonian(g) ==> undirectedHamiltonian(f(g))
+
+    lemma reduction_lemma_right(g: Graph)
+        requires validGraph(g)
+        requires directedHamiltonianCircuit(g)
+        ensures undirectedHamiltonianCircuit(directed_to_undirected_graph(g))
+    {
+        var g' := directed_to_undirected_graph(g);
+
+        assert |g'|>2;
+        var dhc :| isDirectedHamiltonianCircuit(g, dhc);
+
+        // directedHamiltonianCircuitProperty_lemma(g, dhc);
+        assert forall i :: 0<i<|g| ==> g[dhc[i-1]][dhc[i]] && g[dhc[|g|-1]][dhc[0]];
+
+        var dhc_eq := circuit_equivalence(g, g', dhc);
+
+        // var dhc_uEq := circuit_equivalence(g, g', dhc);
+        // circuit_equivalent_lemma(g, g', dhc, dhc_uEq);
+
+        // assert forall i :: 0<i<|g| ==> (g[dhc[i-1]][dhc[i]] ==> g'[dhc[i-1]+|g|][dhc[i]+|g|*2]);
+        // assert forall i :: 0<i<|g| ==> (g[dhc[i-1]][dhc[i]] ==> g'[dhc[i-1]+|g|][dhc[i]+|g|*2]);
+        // assert g[dhc[|g|-1]][dhc[0]] ==> g'[dhc[|g|-1]+|g|][dhc[0]+|g|*2];
+        
+    }
+
+    // ghost predicate circuit_equivalent(g: Graph, g': Graph, circuit: seq<nat>, circuit': seq<nat>)
+    //     requires validGraph(g)
+    //     requires |g|>2
+    //     requires isDirectedHamiltonianCircuit(g, circuit)
+    //     requires g' == directed_to_undirected_graph(g)
+    //     // ensures forall i :: (0<=i<|circuit'| && i % 3 ==1)  ==> circuit'[i] == circuit[(i-1)/3]
+    // {
+    //     |circuit'|==|g|*3
+    //     &&
+    //     (
+    //         forall i :: 0<=i<|g| ==>    //giving the index of the original node i, the index of the same node in circuit': f(i)=3i+1
+    //         (
+    //             circuit'[i*3]==circuit[i]+|g|*2 //in node
+    //             &&
+    //             circuit'[i*3+1]==circuit[i] //central (original) node
+    //             &&
+    //             circuit'[i*3+2]==circuit[i]+|g| //out node
+    //         )
+    //     )
+    // }
+
+    // lemma circuit_equivalent_aux1_lemma(g: Graph, g': Graph, circuit: seq<nat>, circuit': seq<nat>)
+    //     requires validGraph(g)
+    //     requires |g|>2
+    //     requires isDirectedHamiltonianCircuit(g, circuit)
+    //     requires g' == directed_to_undirected_graph(g)
+    //     requires circuit_equivalent(g, g', circuit, circuit')
+    //     ensures forall i :: 0<=i<|circuit'| ==> circuit'[i]<|g'|
+    // {
+    //     forall i | 0<=i<|circuit'|
+    //     {
+    //         circuit_equivalent_aux1_local_lemma(g, g', circuit, circuit', i);
+    //     }
+    // }
+
+    // lemma circuit_equivalent_aux1_local_lemma(g: Graph, g': Graph, circuit: seq<nat>, circuit': seq<nat>, i: int)
+    //     requires validGraph(g)
+    //     requires |g|>2
+    //     requires isDirectedHamiltonianCircuit(g, circuit)
+    //     requires g' == directed_to_undirected_graph(g)
+    //     requires circuit_equivalent(g, g', circuit, circuit')
+    //     requires 0<=i<|circuit'|
+    //     ensures circuit'[i]<|g'|
+    // {
+    //     assert circuit'[i*3]==circuit[i]+|g|*2;
+    //     assert circuit'[i*3+1]==circuit[i];
+    //     assert circuit'[i*3+2]==circuit[i]+|g|;
+    // }
+
+    // lemma circuit_equivalent_lemma(g: Graph, g': Graph, circuit: seq<nat>, circuit': seq<nat>)
+    //     requires validGraph(g)
+    //     requires |g|>2
+    //     requires isDirectedHamiltonianCircuit(g, circuit)
+    //     requires g' == directed_to_undirected_graph(g)
+    //     requires circuit_equivalent(g, g', circuit, circuit')
+    //     ensures isUndirectedHamiltonianCircuit(g', circuit')
+    // {
+    //     if !isUndirectedHamiltonianCircuit(g', circuit')
+    //     {
+    //         reveal circuit_equivalent(g, g', circuit, circuit');
+    //         directedHamiltonianCircuitProperty_lemma(g, circuit);
+    //         assert forall i :: 0<i<|g| ==> g[circuit[i-1]][circuit[i]]; //property_lemma definition
+    //         assert forall i :: 0<=i<|g| ==> circuit'[i*3+1]==circuit[i] && circuit'[i*3]==circuit[i]+|g|*2 && circuit'[i*3+2]==circuit[i]+|g|;  //equivalence property
+    //         assert forall i :: 0<=i<|g| ==> 0<=circuit[i]<|g|;
+    //         assert forall i :: 0<=i<|g| ==> g'[circuit'[i*3+1]][circuit'[i*3]];
+    //     }
+    // }
+
+    //returns the directed circuit's undirected equivalence
+    ghost function circuit_equivalence(g: Graph, g': Graph, circuit: seq<nat>): seq<nat>
+        requires validGraph(g)
+        requires |g|>2
+        requires isDirectedHamiltonianCircuit(g, circuit)
+        requires g' == directed_to_undirected_graph(g)
+        ensures isUndirectedHamiltonianCircuit(g', circuit_equivalence(g, g', circuit))
+    {
+        circuit_equivalence_connectivity_lemma(g, g', circuit, |g|-1);
+        circuit_equivalence_(g, g', circuit, |g|-1)
+    }
+
+    ghost function circuit_equivalence_(g: Graph, g': Graph, circuit: seq<nat>, i: int): seq<nat>
+        requires validGraph(g)
+        requires |g|>2
+        requires isDirectedHamiltonianCircuit(g, circuit)
+        requires g' == directed_to_undirected_graph(g)
+        requires -1<=i<|circuit|
+        decreases i
+        //size relation
+        ensures |circuit_equivalence_(g, g', circuit, i)| == (i+1)*3
+        ensures |circuit_equivalence_(g, g', circuit, i)| % 3 == 0 //triplets
+        // ensures |circuit_equivalence_(g, g', circuit, i)| == |circuit_equivalence_(g, g', circuit, i-1)|+3
+        //central, in and out nodes position relation
+        ensures forall j :: 0<=j<= i ==> 
+        (
+            circuit_equivalence_(g, g', circuit, i)[3*j] == circuit[j]+|g|*2
+            &&
+            circuit_equivalence_(g, g', circuit, i)[3*j+1] == circuit[j]
+            &&
+            circuit_equivalence_(g, g', circuit, i)[3*j+2] == circuit[j]+|g|
+        )
+        //reverse relation
+        ensures i>=0 ==>
+        (
+            var circuit' := circuit_equivalence_(g, g', circuit, i);
+            circuit'[|circuit'|-3] == circuit[(|circuit'|-3)/3]+|g|*2
+            &&
+            circuit'[|circuit'|-2] == circuit[((|circuit'|-2)-1)/3]
+            &&
+            circuit'[|circuit'|-1] == circuit[((|circuit'|-1)-2)/3]+|g|
+        )
+        // ensures forall j :: 0<=j<|circuit_equivalence_(g, g', circuit, i)| ==>
+        // (
+        //     (j % 3 == 0 ==> (circuit_equivalence_(g, g', circuit, i)[j] == circuit[(j)/3]+|g|*2))
+        //     &&
+        //     (j % 3 == 1 ==> (circuit_equivalence_(g, g', circuit, i)[j] == circuit[(j-1)/3]))
+        //     &&
+        //     (j % 3 == 2 ==> (circuit_equivalence_(g, g', circuit, i)[j] == circuit[(j-2)/3]+|g|))
+        // )
+        //nodes boundaries
+        ensures forall j :: 0<j<|circuit_equivalence_(g, g', circuit, i)| ==> circuit_equivalence_(g, g', circuit, i)[j]<|g'|
+        //connectivity
+        // ensures var circuit' := circuit_equivalence_(g, g', circuit, i);
+            // forall j :: 0<j<|circuit'| ==> g'[circuit'[j-1]][circuit'[j]]
+    {
+        if i==-1 then [] else
+            var circuit' := circuit_equivalence_(g, g', circuit, i-1);
+            var ret_circuit := circuit' + [circuit[i]+|g|*2] + [circuit[i]] + [circuit[i]+|g|];
+            // assert |ret_circuit| == |circuit'|+3;
+            // var i1, i2, i3 := |circuit'|, |circuit'|+1, |circuit'|+2;
+            // assert ret_circuit[i1] == circuit[(i1)/3]+|g|*2;
+            // assert ret_circuit[i2] == circuit[(i2-1)/3];
+            // assert ret_circuit[i3] == circuit[(i3-2)/3]+|g|;
+            ret_circuit
+    }
+
+    lemma circuit_equivalence_reverse_position_relation_lemma(g: Graph, g': Graph, circuit: seq<nat>, i: int)
+        requires validGraph(g)
+        requires |g|>2
+        requires isDirectedHamiltonianCircuit(g, circuit)
+        requires g' == directed_to_undirected_graph(g)
+        requires -1<=i<|circuit|
+        ensures var circuit' := circuit_equivalence_(g, g', circuit, i);
+            forall j :: 0<=j<|circuit'| ==>
+            (
+                (j % 3 == 0 ==> (circuit'[j] == circuit[(j)/3]+|g|*2))
+                &&
+                (j % 3 == 1 ==> (circuit'[j] == circuit[(j-1)/3]))
+                &&
+                (j % 3 == 2 ==> (circuit'[j] == circuit[(j-2)/3]+|g|))
+            )
+    {
+        if i>0
+        {
+            circuit_equivalence_reverse_position_relation_lemma(g, g', circuit, i-1);
+            var circuit1 := circuit_equivalence_(g, g', circuit, i-1);
+            var circuit2 := circuit_equivalence_(g, g', circuit, i);
+            assert circuit2 == circuit_equivalence_(g, g', circuit, i-1) + [circuit[i]+|g|*2] + [circuit[i]] + [circuit[i]+|g|];
+            assert forall j :: 0<=j<|circuit1| ==>
+            (
+                (j % 3 == 0 ==> (circuit1[j] == circuit[(j)/3]+|g|*2))
+                &&
+                (j % 3 == 1 ==> (circuit1[j] == circuit[(j-1)/3]))
+                &&
+                (j % 3 == 2 ==> (circuit1[j] == circuit[(j-2)/3]+|g|))
+            );
+            var j1, j2, j3 := |circuit2|-3, |circuit2|-2, |circuit2|-1;
+            assert j1%3==0 && j2%3==1 && j3%3==2;
+            // assert
+            // (
+            //     (j1 % 3 == 0 && (circuit1[j1] == circuit[(j1)/3]+|g|*2))
+            //     &&
+            //     (j2 % 3 == 1 && (circuit1[j2] == circuit[(j2-1)/3]))
+            //     &&
+            //     (j3 % 3 == 2 && (circuit1[j3] == circuit[(j3-2)/3]+|g|))
+            // );
+            assume forall j :: 0<=j<|circuit2| ==>
+            (
+                (j % 3 == 0 ==> (circuit2[j] == circuit[(j)/3]+|g|*2))
+                &&
+                (j % 3 == 1 ==> (circuit2[j] == circuit[(j-1)/3]))
+                &&
+                (j % 3 == 2 ==> (circuit2[j] == circuit[(j-2)/3]+|g|))
+            );
+        }
+    }
+
+    lemma circuit_equivalence_connectivity_lemma(g: Graph, g': Graph, circuit: seq<nat>, i: int)
+        requires validGraph(g)
+        requires |g|>2
+        requires isDirectedHamiltonianCircuit(g, circuit)
+        requires g' == directed_to_undirected_graph(g)
+        requires 0<=i<|circuit|
+        ensures var circuit' := circuit_equivalence_(g, g', circuit, i);
+            (forall j :: 0<j<|circuit'| ==> g'[circuit'[j-1]][circuit'[j]]) && g'[circuit'[|circuit'|-1]][circuit'[0]]
+    // {
+    //     var circuit' := circuit_equivalence_(g, g', circuit, i);
+    //     forall j | 0<j<|circuit'|
+    //     {
+    //         circuit_equivalence_connectivity_local_lemma(g, g', circuit, i, circuit', j);
+    //     }
+    // }
+
+    // lemma circuit_equivalence_connectivity_local_lemma(g: Graph, g': Graph, circuit: seq<nat>, i: int, circuit': seq<nat>, j: int)
+    //     requires validGraph(g)
+    //     requires |g|>2
+    //     requires isDirectedHamiltonianCircuit(g, circuit)
+    //     requires g' == directed_to_undirected_graph(g)
+    //     requires 0<=i<|circuit|
+    //     requires circuit' == circuit_equivalence_(g, g', circuit, i)
+    //     requires 0<j<|circuit'|
+    //     ensures g'[circuit'[j-1]][circuit'[j]]
+    // {
+    //     if j%3==0
+    //     {
+    //         // assert circuit'[j] == circuit[j]+|g|*2;
+    //         assume g'[circuit'[j-1]][circuit'[j]];
+    //     }
+    //     if j%3==1
+    //     {assume g'[circuit'[j-1]][circuit'[j]];}
+    //     if j%3==2
+    //     {assume g'[circuit'[j-1]][circuit'[j]];}
+    // }
+
+    // Reduction to the left: undirectedHamiltonian(f(g)) ==> directedHamiltonian(g)
+
+    lemma reduction_lemma_left(g: Graph) //TODO
+        requires validGraph(g)
+        requires undirectedHamiltonianCircuit(directed_to_undirected_graph(g))
+        ensures directedHamiltonianCircuit(g)
+    // {}
+
+
+    // ghost function directedHamiltonianCircuit_witness(g: Graph): seq<nat>
+    //     requires validGraph(g)
+    //     requires directedHamiltonianCircuit(g)
+    //     ensures isDirectedHamiltonianCircuit(g, (directedHamiltonianCircuit_witness(g)))
+
+    // ghost function undirectedHamiltonianCircuit_witness(g: Graph): seq<nat>
+    //     requires validUndirectedGraph(g)
+    //     requires undirectedHamiltonianCircuit(g)
+    //     ensures isUndirectedHamiltonianCircuit(g, (undirectedHamiltonianCircuit_witness(g)))
+
+}
