reduction_directedHamiltonianCircuit_to_hamiltonianCircuit/reduction_hamiltonian_rFunction.dfy
@@ -1,0 +1,229 @@
+include "reduction_hamiltonian_definitions.dfy"
+
+module ReductionFunction
+{
+    import opened Definitions
+
+    /***************
+    REDUCTION: DIRECTED HAMILTONIAN <p UNDIRECTED HAMILTONIAN
+    ****************/
+
+    /////// AUXILIAR PREDICATES //////
+
+    ghost predicate unconnected_graph(g: Graph)
+        requires validGraph(g)
+    {
+        forall f :: 0<=f<|g| ==> (forall c :: 0<=c<|g| ==> !g[f][c])
+    }
+
+    //original nodes are only adjacent to their respective out and in nodes and there are only out->in vertex
+    ghost predicate in_out_graph(g: Graph, s: int)
+        requires validUndirectedGraph(g)
+        requires |g|==s*3
+    {
+        forall f :: 0<=f< s ==> (forall c :: 0<=c<|g| ==>
+            (
+                ((c==f+s || c==f+s*2) ==> g[f][c])     //out node: i+s, in node: i+s*2
+                &&
+                ((c!=f+s && c!=f+s*2) ==> !g[f][c])    //rest: false (original nodes are not interconnected)
+            )
+        )
+        &&
+        (forall f :: s<=f< s*2 ==> (forall c :: s<=c< s*2 ==> !g[f][c]))    //no vertex from out to out
+        &&
+        (forall f :: s*2<=f< s*3 ==> (forall c :: s*2<=c< s*3 ==> !g[f][c]))    //no vertex from in to in
+    }
+
+    ghost predicate unconnected_in_out_graph(g: Graph, s: int)
+        requires validUndirectedGraph(g)
+        requires |g|==s*3
+    {
+        in_out_graph(g, s)
+        &&
+        forall f :: s<=f<|g| ==> (forall c :: 0<=c<|g| ==> !g[f][c])
+    }
+
+    ghost predicate out_node_unconnected(g: Graph, g0: Graph, n: int)
+        requires validUndirectedGraph(g)
+        requires |g|==|g0|*3
+        requires 0<=n< |g0|
+    {
+        forall c :: 0<=c< |g| ==> !g[n+|g0|][c] //no vertex for n_out node
+    }
+
+    /////// REDUCTION FUNCTION ///////
+
+    ghost opaque function directed_to_undirected_graph(g: Graph): Graph
+        requires validGraph(g)
+        //size relation: 2 extra nodes (node_in and node_out) per node
+        ensures |directed_to_undirected_graph(g)| == |g|*3
+        //squared and triangular superior matrix
+        ensures validUndirectedGraph(directed_to_undirected_graph(g))
+        //original nodes are only adjacent to their respective out and in nodes and there are only out->in vertex
+        ensures in_out_graph(directed_to_undirected_graph(g), |g|)
+        //direction relation: n1->n2 in g only and only if n1_out-n2_in in g'
+        ensures forall f :: 0<=f<|g| ==> (forall c :: 0<=c<|g| ==> (g[f][c] <==> directed_to_undirected_graph(g)[f+|g|][c+|g|*2]))
+    {
+        if |g|==0 then g else direction_equivalence(g, in_out_nodes(extended_graph(g), |g|))
+    }
+
+    ghost function extended_graph(g: Graph): Graph
+        requires validGraph(g)
+        requires |g|>0
+        ensures validUndirectedGraph(extended_graph(g))
+        ensures |extended_graph(g)|==|g|*3    //original nodes +2 nodes per original node (nodeIn and nodeOut)
+        ensures unconnected_graph(extended_graph(g))
+    {
+        seq(|g|*3, i => seq(|g|*3, i => false))
+    }
+
+    ghost function in_out_nodes(g: Graph, s: int): Graph
+        requires validUndirectedGraph(g)
+        requires unconnected_graph(g)
+        // requires |g|>0
+        requires |g|==s*3
+        ensures |in_out_nodes(g, s)| == |g|
+        ensures validUndirectedGraph(in_out_nodes(g, s))
+        ensures unconnected_in_out_graph(in_out_nodes(g, s), s)
+    {
+        in_out_nodes_(g, s, s-1)
+    }
+
+    ghost function in_out_nodes_(g: Graph, s: int, i: int): Graph
+        requires validUndirectedGraph(g)
+        requires forall f :: 0<=f<|g| ==> (forall c :: 0<=c<|g| ==> !g[f][c])
+        // requires |g|>0
+        requires |g|==s*3
+        requires -1<=i< s
+        decreases i
+        ensures |in_out_nodes_(g, s, i)| == |g|
+        ensures validUndirectedGraph(in_out_nodes_(g, s , i))
+        ensures forall f :: i< f<|g| ==> (forall c :: 0<=c<|g| ==> !in_out_nodes_(g, s, i)[f][c])
+        ensures forall f :: 0<=f<=i ==> (forall c :: 0<=c<|g| ==>
+            (
+                ((c==f+s || c==f+s*2) ==> in_out_nodes_(g, s, i)[f][c])     //out node: i+s, in node: i+s*2
+                &&
+                ((c!=f+s && c!=f+s*2) ==> !in_out_nodes_(g, s, i)[f][c])    //rest: false
+            )
+        )
+    {
+        if i==-1 then g else
+            var g' := in_out_nodes_(g, s, i-1);
+            var f := g'[i];
+            var f' := f[..i+s] + [true] + f[i+s+1..];           //out node
+            var f'' := f'[..i+s*2] + [true] + f'[i+s*2+1..];    //in node
+            g'[i:=f'']
+    }
+
+    ghost function direction_equivalence(g: Graph, g': Graph): Graph
+        requires |g|>0
+        requires validGraph(g)
+        requires validUndirectedGraph(g')
+        requires |g'|==|g|*3
+        requires unconnected_in_out_graph(g', |g|)
+        //size persistence
+        ensures |direction_equivalence(g, g')| == |g'|
+        //squared and triangular superior matrix
+        ensures validUndirectedGraph(direction_equivalence(g, g'))
+        //original nodes are only adjacent to their respective out and in nodes and there are only out->in vertex
+        ensures in_out_graph(direction_equivalence(g, g'), |g|)
+        //modifying property: n1->n2 in g only and only if n1_out-n2_in in g'
+        ensures forall f :: 0<=f<|g| ==> (forall c :: 0<=c<|g| ==> (g[f][c] <==> direction_equivalence(g, g')[f+|g|][c+|g|*2]))
+    {
+        direction_equivalence_(g, g', |g|-1)
+    }
+
+    ghost function direction_equivalence_(g: Graph, g': Graph, i: int): Graph
+        requires |g|>0
+        requires validGraph(g)
+        requires validUndirectedGraph(g')
+        requires |g'|==|g|*3
+        requires -1<=i<|g|
+        requires unconnected_in_out_graph(g', |g|)
+        ensures |direction_equivalence_(g, g', i)| == |g'|
+        ensures validUndirectedGraph(direction_equivalence_(g, g', i))
+        //only out nodes are modified (original nodes and in nodes stay the same)
+        ensures forall f :: 0<=f<|g| ==> (g'[f] == direction_equivalence_(g, g', i)[f])
+        ensures forall f :: |g|*2<=f<|g'| ==> (g'[f] == direction_equivalence_(g, g', i)[f])
+        //only out to in vertex are modified so vertex in the range [0]..[|g|*2-1] stay the same
+        ensures forall f :: |g|<=f<|g|*2 ==> (forall c :: 0<=c<|g|*2 ==> (g'[f][c] == direction_equivalence_(g, g', i)[f][c]))
+        //inductive postconditions
+        //every row yet to process stay the same
+        ensures forall f :: i+|g|< f<|g'| ==> (g'[f] == direction_equivalence_(g, g', i)[f])
+        //modifying property: for every processed row: n_out to c_in in g' if and only if n to c in g
+        ensures forall f :: 0<=f<=i ==> (forall c :: 0<=c<|g| ==> (g[f][c] <==> direction_equivalence_(g, g', i)[f+|g|][c+|g|*2]))
+    {
+        if i==-1 then g' else
+            var g'' := direction_equivalence_(g, g', i-1);
+            //recorrer fila: si columna es true entonces [fila+s](out)[columna+s*2](in) := true
+            var gF := direction_equivalence_node(g, g'', i);
+            gF
+    }
+
+    ghost function direction_equivalence_node(g: Graph, g': Graph, n: int): Graph
+        requires |g|>0
+        requires validGraph(g)
+        requires validUndirectedGraph(g')
+        requires |g'|==|g|*3
+        requires 0<=n<|g|
+        requires out_node_unconnected(g', g, n)
+        ensures |direction_equivalence_node(g, g', n)| == |g'|
+        ensures validUndirectedGraph(direction_equivalence_node(g, g', n))
+        //only n_out's row is modified
+        ensures forall f :: 0<=f<|g'| && f!=n+|g| ==> (g'[f] == direction_equivalence_node(g, g', n)[f])
+        //only n_out to x_in vertex are modified, so columns below n+|g|*2 stay the same (set to false)
+        ensures forall c :: 0<=c<|g|*2 ==> (g'[n+|g|][c] == direction_equivalence_node(g, g', n)[n+|g|][c])
+        ensures forall c :: 0<=c<|g|*2 ==> !direction_equivalence_node(g, g', n)[n+|g|][c]
+        //modifying property: n_out to c_in in g' if and only if n to c in g
+        ensures forall c :: 0<=c<|g| ==> (g[n][c] <==> direction_equivalence_node(g, g', n)[n+|g|][c+|g|*2])
+    {
+        direction_equivalence_node_(g, g', n, |g|-1)
+    }
+
+    /**
+    columna i del nodo n en g:
+        si [n][i] true : hay una arista de n a i -> [n_out][i_in] := true : [n+s][i+s*2]:=true
+        Nota:
+            es importante el orden [n_out][n_in] porque los nodos out tienen un valor menor que los nodos in
+            (n_out: n+s y n_in n+s*2 siendo n su nodo central) por lo que si fuese a la inversa no se conservaría
+            la propiedad de matriz triangular superior utilizada, en este caso, para categorizar grafos no dirigidos.
+    */
+    ghost function direction_equivalence_node_(g: Graph, g': Graph, n: int, i: int): Graph
+        requires |g|>0
+        requires validGraph(g)
+        requires validUndirectedGraph(g')
+        requires |g'|==|g|*3
+        requires 0<=n<|g|
+        requires -1<=i<|g|
+        requires out_node_unconnected(g', g, n)
+        ensures |direction_equivalence_node_(g, g', n, i)| == |g'|
+        ensures validUndirectedGraph(direction_equivalence_node_(g, g', n, i))
+        //only n_out's row is modified
+        ensures forall f :: 0<=f<|g'| && f!=n+|g| ==> (g'[f] == direction_equivalence_node_(g, g', n, i)[f])
+        //only n_out -> x_in vertex are modified, so columns below n+|g|*2 stay the same
+        ensures forall c :: 0<=c<|g|*2 ==> (g'[n+|g|][c] == direction_equivalence_node_(g, g', n, i)[n+|g|][c])
+        //inductive postconditions:
+        //every column yet to process stays the same (set to false)
+        ensures forall f :: i+|g|*2< f<|g'| ==> (g'[n+|g|][f] == direction_equivalence_node_(g, g', n, i)[n+|g|][f])
+        ensures forall f :: i< f<|g| ==> (g'[n+|g|][f+|g|*2] == direction_equivalence_node_(g, g', n, i)[n+|g|][f+|g|*2])
+        ensures forall f :: i< f<|g| ==> !direction_equivalence_node_(g, g', n, i)[n+|g|][f+|g|*2]
+        //modifying property: n_out to i_in in g' if and only if n to c in g
+        ensures forall c :: 0<=c<=i ==>
+        (
+            g[n][c] <==> direction_equivalence_node_(g, g', n, i)[n+|g|][c+|g|*2]
+        )
+    {
+        if i==-1 then
+            g'
+        else
+            var g'' := direction_equivalence_node_(g, g', n, i-1);
+            if g[n][i] then
+                var f_aux1 := g''[n+|g|];
+                var f_aux2 := f_aux1[..i+|g|*2]+[true]+f_aux1[i+|g|*2+1..];
+                var gF := g''[n+|g| := f_aux2];
+                gF
+            else
+                g''
+    }
+
+}
